Refactored inftraces out of fairness file

fairness/fairness.v
@@ -1,236 +1,7 @@
-From trillium.program_logic Require Export adequacy.
 From stdpp Require Import option.
 From Paco Require Import paco1 paco2 pacotac.
-
-Require Import
-        Coq.Relations.Relation_Definitions
-        Coq.Relations.Relation_Operators.
-Require Import Coq.Arith.Wf_nat.
-
-Section traces.
-
-  Delimit Scope trace_scope with trace.
-
-  CoInductive trace (S L: Type) :=
-  | tr_singl (s: S)
-  | tr_cons (s: S) (ℓ: L) (r: trace S L).
-  Bind Scope trace_scope with trace.
-
-  Arguments tr_singl {_} {_}, _.
-  Arguments tr_cons {_} {_} _ _ _%trace.
-  Notation "⟨ s ⟩" := (tr_singl s) : trace_scope.
-  Notation "s -[ ℓ ]->  r" := (tr_cons s ℓ r) (at level 33) : trace_scope.
-  Open Scope trace.
-
-  Lemma trace_unfold_fold {S L} (tr: trace S L) :
-    tr = match tr with
-         | ⟨s⟩ => ⟨s⟩
-         | s -[ℓ]-> rest => s -[ℓ]-> rest
-         end.
-  Proof. destruct tr; trivial. Qed.
-
-  Definition trfirst {S L} (tr: trace S L): S :=
-    match tr with
-    | ⟨s⟩ => s
-    | s -[ℓ]-> r => s
-    end.
-
-  Lemma pred_first_trace (S T : Type) (tr: trace S T ) (P: S -> Prop):
-    match tr with
-    | ⟨ s ⟩ | s -[ _ ]-> _ => P s
-    end <-> P (trfirst tr).
-  Proof. destruct tr; done. Qed.
-
-  Section after.
-    Context {St L: Type}.
-
-    Fixpoint after (n: nat) (t: trace St L) : option (trace St L):=
-      match n with
-      | 0 => Some t
-      | Datatypes.S n =>
-        match t with
-        | ⟨ s ⟩ => None
-        | s -[ ℓ ]-> xs => after n xs
-        end
-      end.
-
-    Definition pred_at (tr: trace St L) (n: nat) (P: St -> option L -> Prop): Prop :=
-      match after n tr with
-      | None => False
-      | Some ⟨s⟩ => P s None
-      | Some (s -[ℓ]-> _) => P s (Some ℓ)
-      end.
-
-    Lemma after_sum m: forall k (tr: trace St L),
-        after (k+m) tr =
-        match after m tr with
-        | None => None
-        | Some tr' => after k tr'
-        end.
-    Proof.
-      induction m.
-      - intros k tr. by have ->: k+0=k by lia.
-      - intros k tr. simpl.
-        have -> /=: (k + S m) = S (k+m) by lia.
-        destruct tr as [s|s l r]; simpl; auto.
-    Qed.
-
-    Lemma after_sum' m: forall k (tr: trace St L),
-        after (k+m) tr =
-        match after k tr with
-        | None => None
-        | Some tr' => after m tr'
-        end.
-    Proof. intros. rewrite Nat.add_comm. apply after_sum. Qed.
-
-    Lemma pred_at_sum P n m tr:
-      pred_at tr (n + m) P <->
-      match after n tr with
-      | None => False
-      | Some tr' => pred_at tr' m P
-      end.
-    Proof.
-      rewrite /pred_at after_sum'.
-        by destruct (after n tr).
-    Qed.
-
-    Lemma pred_at_sum' P n m tr:
-      pred_at tr (n + m) P <->
-      match after m tr with
-      | None => False
-      | Some tr' => pred_at tr' n P
-      end.
-    Proof.
-      rewrite /pred_at after_sum.
-        by destruct (after m tr).
-    Qed.
-
-    Lemma pred_at_0 s ℓ r P:
-      pred_at (s -[ℓ]-> r) 0 P <-> P s (Some ℓ).
-    Proof. by unfold pred_at. Qed.
-
-    Lemma pred_at_S s ℓ r n P:
-      pred_at (s -[ℓ]-> r) (S n) P <-> pred_at r n P.
-    Proof. by unfold pred_at. Qed.
-
-    Definition infinite_trace tr :=
-      forall n, is_Some (after n tr).
-
-    Definition terminating_trace tr :=
-      ∃ n, after n tr = None.
-
-    Lemma terminating_trace_cons s ℓ tr:
-      terminating_trace tr -> terminating_trace (s -[ℓ]-> tr).
-    Proof. intros [n Hterm]. by exists (1+n). Qed.
-
-    Lemma infinite_trace_after n tr:
-      infinite_trace tr -> match after n tr with
-                          | None => False
-                          | Some tr' => infinite_trace tr'
-                          end.
-    Proof.
-      intros Hinf. have [tr' Htr'] := (Hinf n). rewrite Htr'.
-      intros m.
-      have Hnm := Hinf (n+m). rewrite after_sum' Htr' // in Hnm.
-    Qed.
-
-    Lemma infinite_cons s ℓ r:
-      infinite_trace (s -[ℓ]-> r) -> infinite_trace r.
-    Proof.
-      intros Hinf n. specialize (Hinf (1+n)).
-      rewrite (after_sum' _ 1) // in Hinf.
-    Qed.
-  End after.
-
-End traces.
-
-Delimit Scope trace_scope with trace.
-Arguments tr_singl {_} {_}, _.
-Arguments tr_cons {_} {_} _ _ _%trace.
-Notation "⟨ s ⟩" := (tr_singl s) : trace_scope.
-Notation "s -[ ℓ ]->  r" := (tr_cons s ℓ r) (at level 33) : trace_scope.
-Open Scope trace.
-
-Section simulation.
-  Context {L1 L2 S1 S2: Type}.
-  Context (Rℓ: L1 -> L2 -> Prop) (Rs: S1 -> S2 -> Prop).
-  Context (trans1: S1 -> L1 -> S1 -> Prop).
-  Context (trans2: S2 -> L2 -> S2 -> Prop).
-
-  CoInductive traces_match : trace S1 L1 -> trace S2 L2 -> Prop :=
-  | trace_match_singl s1 s2: Rs s1 s2 -> traces_match ⟨ s1 ⟩ ⟨ s2 ⟩
-  | trace_match_cons s1 ℓ1 r1 s2 ℓ2 r2 : Rℓ ℓ1 ℓ2 -> Rs s1 s2 ->
-                                         trans1 s1 ℓ1 (trfirst r1) ->
-                                         trans2 s2 ℓ2 (trfirst r2) ->
-                                         traces_match r1 r2 ->
-                                         traces_match (s1 -[ℓ1]-> r1) (s2 -[ℓ2]-> r2).
-
-  Lemma traces_match_after tr1 tr2 n tr2':
-    traces_match tr1 tr2 ->
-    after n tr2 = Some tr2' ->
-    (exists tr1', after n tr1 = Some tr1' ∧ traces_match tr1' tr2').
-  Proof.
-    revert tr1 tr2.
-    induction n; intros tr1 tr2.
-    { simpl. intros. exists tr1. simplify_eq. done. }
-    move=> /= Hm Ha. destruct tr2 as [|s ℓ tr2''] eqn:Heq; first done.
-    destruct tr1; first by inversion Hm.
-    inversion Hm; simplify_eq. by eapply IHn.
-  Qed.
-
-  Lemma traces_match_first tr1 tr2:
-    traces_match tr1 tr2 ->
-    Rs (trfirst tr1) (trfirst tr2).
-  Proof. intros Hm. inversion Hm; done. Qed.
-
-End simulation.
-
-Section execs_and_traces.
-  Context {S L: Type}.
-
-  CoInductive exec_trace_match: finite_trace S L -> inflist (L * S) -> trace S L -> Prop :=
-  | exec_trace_match_singl ft s: trace_last ft = s -> exec_trace_match ft infnil ⟨s⟩
-  | exec_trace_match_cons ft s ℓ ift tr:
-      exec_trace_match (trace_extend ft ℓ s) ift tr ->
-      exec_trace_match ft (infcons (ℓ, s) ift) (trace_last ft -[ℓ]-> tr).
-
-  CoFixpoint to_trace (s: S) (il: inflist (L * S)) : trace S L :=
-    match il with
-    | infnil => ⟨ s ⟩
-    | infcons (ℓ, s') rest => s -[ℓ]-> (to_trace s' rest)
-    end.
-
-  Lemma to_trace_spec (fl: finite_trace S L) (il: inflist (L * S)):
-    exec_trace_match fl il (to_trace (trace_last fl) il).
-  Proof.
-    revert fl il. cofix CH. intros s il.
-    rewrite (trace_unfold_fold (to_trace _ il)). destruct il as [| [ℓ x]?]; simpl in *.
-    - by econstructor.
-    - econstructor. have ->: x = trace_last (trace_extend s ℓ x) by done.
-      apply CH.
-  Qed.
-
-  Lemma to_trace_singleton s (il: inflist (L * S)):
-    exec_trace_match (trace_singleton s) il (to_trace s il).
-  Proof. apply to_trace_spec. Qed.
-
-  CoFixpoint from_trace (tr: trace S L): inflist (L * S) :=
-    match tr with
-    | ⟨ s ⟩ => infnil
-    | s -[ℓ]-> tr' => infcons (ℓ, trfirst tr') (from_trace tr')
-    end.
-
-  Lemma from_trace_spec (fl: finite_trace S L) (tr: trace S L):
-    trace_last fl = trfirst tr ->
-    exec_trace_match fl (from_trace tr) tr.
-  Proof.
-    revert fl tr. cofix CH. intros fl tr Heq.
-    rewrite (inflist_unfold_fold (from_trace tr)). destruct tr; simpl in *.
-    - by econstructor.
-    - rewrite -Heq. econstructor. apply CH; done.
-  Qed.
-
-End execs_and_traces.
+From trillium.program_logic Require Export adequacy.
+From trillium.fairness Require Export inftraces.
 
 Record FairModel : Type := {
   fmstate:> Type;
@@ -283,6 +54,7 @@ Section fairness.
   | Silent_step: locale Λ -> FairLabel
   | Config_step: FairLabel
   .
+  Arguments FairLabel : clear implicits.
 
   Definition less (x y: option nat) :=
     match x, y with
@@ -300,21 +72,6 @@ Section fairness.
   | Zombie otid (Hismainrole: oρ = Some ρ') (Hnotalive: ρ' ∉ live_roles _ b) (Hnotdead: ρ' ∈ dom b.(ls_fuel)):
     must_decrease ρ' oρ a b otid
   .
-
-  Definition oleq (a b : option nat) : Prop :=
-    match a, b with
-    | Some x, Some y => x ≤ y
-    | _, _ => False
-    end.
-
-  Definition oless (a b : option nat) : Prop :=
-    match a, b with
-    | Some x, Some y => x < y
-    | _, _ => False
-    end.
-
-  Lemma oleq_oless a b : oless a b -> oleq a b.
-  Proof. destruct a; destruct b=>//. unfold oless, oleq. lia. Qed.
 
   Definition fuel_decr (tid: olocale Λ) (oρ: option M.(fmrole))
              (a b: LiveState) :=
@@ -354,8 +111,8 @@ Section fairness.
   Record LiveModel := {
       lm_fl : M → nat;
       lm_ls := LiveState;
-      lm_lbl := @FairLabel M.(fmrole);
-      lm_ls_trans := @ls_trans lm_fl;
+      lm_lbl := FairLabel M.(fmrole);
+      lm_ls_trans := ls_trans lm_fl;
     }.
   
   Definition fair_model_model `(LM : LiveModel) : Model := {|
@@ -478,9 +235,7 @@ End exec_trace.
 Definition auxtrace `(LM: LiveModel Λ M) := trace LM.(lm_ls) LM.(lm_lbl).
 
 Section aux_trace.
-  Context {Λ: language}.
-  Context {M: FairModel}.
-  Context {LM: LiveModel Λ M}.
+  Context `{LM: LiveModel Λ M}.
 
   Definition role_enabled ρ (δ: LiveState Λ M) := ρ ∈ M.(live_roles) δ.
 
@@ -523,80 +278,6 @@ Section aux_trace.
 
 End aux_trace.
 
-(* Adapted from Arthur Azevedo De Amorim *)
-Section lex_ind.
- Section Lexicographic.
-
-   Variables (A B : Type) (leA : relation A) (leB : relation B).
-
-   Inductive lexprod : A * B -> A * B -> Prop :=
-   | left_lex  : forall x x' y y', leA x x' -> lexprod (x, y) (x', y')
-   | right_lex : forall x y y',    leB y y' -> lexprod (x, y) (x, y').
-
-   Theorem wf_trans :
-     transitive _ leA ->
-     transitive _ leB ->
-     transitive _ lexprod.
-   Proof.
-     intros tA tB [x1 y1] [x2 y2] [x3 y3] H.
-     inversion H; subst; clear H.
-     - intros H.
-       inversion H; subst; clear H; apply left_lex; now eauto.
-    - intros H.
-    inversion H; subst; clear H.
-    + now apply left_lex.
-    + now apply right_lex; eauto.
-    Qed.
-
-    Theorem wf_lexprod :
-    well_founded leA ->
-    well_founded leB ->
-    well_founded lexprod.
-    Proof.
-      intros wfA wfB [x y]. generalize dependent y.
-      induction (wfA x) as [x _ IHx]; clear wfA.
-      intros y.
-      induction (wfB y) as [y _ IHy]; clear wfB.
-      constructor.
-      intros [x' y'] H.
-      now inversion H; subst; clear H; eauto.
-    Qed.
-
- End Lexicographic.
-
- Definition lt_lex : relation (nat * nat) := fun '(x, y) '(x', y') =>
-                                            x < x' ∨ (x = x' ∧ y <= y').
-
- #[global] Instance lt_lex_partial_order : @PartialOrder (nat * nat) lt_lex.
- Proof.
-   constructor.
-   + constructor.
-     * move=> [x y]. right; split; reflexivity.
-     * move=> [x1 y1] [x2 y2] [x3 y3] [H1|H1] [H2|H2]; unfold lt_lex; lia.
-   + move=> [x1 y1] [x2 y2] [?|[??]] [H2|[??]]; f_equal; try lia.
- Qed.
-
- Definition myrel : relation (nat * nat) :=
-    lexprod _ _ lt lt.
-
- Lemma lex_ind:
-   ∀ (n : nat*nat) (P : nat*nat → Prop),
-     (∀ n0 : nat*nat, (∀ m : nat*nat, (strict lt_lex) m n0 → P m) → P n0) → P n.
- Proof.
-   assert (well_founded myrel) as Hwf.
-
-   { apply wf_lexprod; apply lt_wf. }
-   induction n using (well_founded_ind Hwf).
-   intros P HI. apply HI =>//. intros m [Ha Hb].
-   apply H =>//. destruct n as [n1 n2]; destruct m as [m1 m2].
-   unfold strict, lt_lex in *.
-   destruct Ha as [Ha | [Ha1 Ha2]].
-   - constructor 1. done.
-    - rewrite Ha1. constructor 2. lia.
- Qed.
-
-End lex_ind.
-
 Ltac SS :=
   epose proof ls_fuel_dom;
   (* epose proof ls_mapping_dom; *)
@@ -616,9 +297,7 @@ Definition exaux_traces_match `{LM:LiveModel Λ M} `{EqDecision (locale Λ)} :
                LM.(lm_ls_trans).
 
 Section fairness_preserved.
-  Context {M: FairModel}.
-  Context {Λ: language}.
-  Context {LM: LiveModel Λ M}.
+  Context `{LM: LiveModel Λ M}.
   Context `{Countable (locale Λ)}.
 
   Lemma exaux_preserves_validity extr (auxtr : auxtrace LM):
@@ -924,7 +603,7 @@ Section fairness_preserved.
         φ ex atr -> valid_state_evolution_fairness ex atr) ->
     exec_trace_match ex iex progtr ->
     exec_trace_match atr iatr auxtr ->
-    @valid_inf_system_trace _ LM φ ex atr iex iatr ->
+    valid_inf_system_trace φ ex atr iex iatr ->
     exaux_traces_match progtr auxtr.
   Proof.
     intros Hφ1 Hφ2.
@@ -950,60 +629,8 @@ Section fairness_preserved.
   Qed.
 End fairness_preserved.
 
-#[global] Program Instance add_monoid: Monoid Nat.add :=
-  {| monoid_unit := 0 |}.
-Next Obligation. intros ???. apply Nat.add_assoc. Qed.
-Next Obligation. intros ??. apply Nat.add_comm. Qed.
-Next Obligation. intros ?. done. Qed.
-
-Section addition_monoid.
-  Context `{Countable K}.
-
-  Lemma big_addM_leq_forall (X Y: gmap K nat):
-    (∀ k, k ∈ dom X -> oleq (X !! k) (Y !! k)) ->
-    ([^ Nat.add map] k ↦ x ∈ X, x) ≤ ([^ Nat.add map] k ↦ y ∈ Y, y).
-  Proof.
-    revert Y.
-    induction X as [|k v X HXk IH] using map_ind.
-    { intros Y Hx. rewrite big_opM_empty /=. lia. }
-    intros Y Hx. rewrite big_opM_insert //.
-    have Hol: oleq (<[k:=v]> X !! k) (Y !! k) by apply Hx; set_solver.
-    rewrite lookup_insert in Hol.
-    destruct (Y!!k) as [v'|] eqn:Heq; last done.
-    rewrite (big_opM_delete _ Y k v') //.
-    apply plus_le_compat=>//.
-    apply IH=> k' Hin.
-    have ?: k ≠ k'.
-    { intros ->. apply elem_of_dom in Hin. rewrite HXk in Hin. by destruct Hin. }
-    rewrite -(lookup_insert_ne X k k' v) // (lookup_delete_ne Y k) //.
-    apply Hx. set_solver.
-  Qed.
-End addition_monoid.
-
-Section dec_unless.
-  Context {St S' L L': Type}.
-  Context (Us: St -> S').
-  Context (Ul: L -> option L').
-
-  Definition dec_unless Ψ (tr: trace St L) :=
-    ∀ n, match after n tr with
-         | Some ⟨ _ ⟩ | None => True
-         | Some (s -[ℓ]-> tr') =>
-           (∃ ℓ', Ul ℓ = Some ℓ') ∨
-           (Ψ (trfirst tr') < Ψ s ∧ Us s = Us (trfirst tr'))
-         end.
-
-  Lemma dec_unless_next Ψ s ℓ tr (Hdec: dec_unless Ψ (s -[ℓ]-> tr)): dec_unless Ψ tr.
-  Proof.
-    intros n. specialize (Hdec (n+1)). rewrite (after_sum 1) // in Hdec.
-  Qed.
-
-End dec_unless.
-
 Section fuel_dec_unless.
-  Context {Mdl: FairModel}.
-  Context {Λ: language}.
-  Context {LM: LiveModel Λ Mdl}.
+  Context `{LM: LiveModel Λ Mdl}.
   Context `{Countable (locale Λ)}.
 
   Definition Ul (ℓ: LM.(mlabel)) :=
@@ -1067,205 +694,14 @@ Section fuel_dec_unless.
   Qed.
 End fuel_dec_unless.
 
-Section destuttering.
-  Context {St S' L L': Type}.
-  Context (Us: St -> S').
-  Context (Ul: L -> option L').
-
-  Inductive upto_stutter_ind (upto_stutter_coind: trace St L -> trace S' L' -> Prop):
-    trace St L -> trace S' L' -> Prop :=
-  | upto_stutter_singleton s:
-      upto_stutter_ind upto_stutter_coind ⟨s⟩ ⟨Us s⟩
-  | upto_stutter_stutter btr str s ℓ:
-      Ul ℓ = None ->
-      (* (Us s = Us (trfirst btr) -> (or something like this...?) *)
-      Us s = Us (trfirst btr) ->
-      Us s = trfirst str ->
-      upto_stutter_ind upto_stutter_coind btr str ->
-      upto_stutter_ind upto_stutter_coind (s -[ℓ]-> btr) str
-  | upto_stutter_step btr str s ℓ s' ℓ':
-      Us s = s' ->
-      Ul ℓ = Some ℓ' ->
-      upto_stutter_coind btr str ->
-      upto_stutter_ind upto_stutter_coind (s -[ℓ]-> btr) (s' -[ℓ']-> str).
-
-  Definition upto_stutter := paco2 upto_stutter_ind bot2.
-
-  Lemma upto_stutter_mono :
-    monotone2 (upto_stutter_ind).
-  Proof.
-    unfold monotone2. intros x0 x1 r r' IN LE.
-    induction IN; try (econstructor; eauto; done).
-  Qed.
-  Hint Resolve upto_stutter_mono : paco.
-
-  Lemma upto_stutter_after {btr str} n {str'}:
-    upto_stutter btr str ->
-    after n str = Some str' ->
-    ∃ n' btr', after n' btr = Some btr' ∧ upto_stutter btr' str'.
-  Proof.
-    have Hw: ∀ (P: nat -> Prop), (∃ n, P (S n)) -> (∃ n, P n).
-    { intros P [x ?]. by exists (S x). }
-    revert btr str str'. induction n as [|n IH]; intros btr str str' Hupto Hafter.
-    { injection Hafter => <-. clear Hafter. exists 0, btr. done. }
-    revert str' Hafter. punfold Hupto. induction Hupto as
-        [s|btr str s ℓ HUl HUs1 HUs2 Hind IHH|btr str s ℓ s' ℓ' ?? Hind].
-    - intros str' Hafter. done.
-    - intros str' Hafter.
-      apply Hw. simpl. by apply IHH.
-    - intros str' Hafter. simpl in Hafter.
-      apply Hw. simpl. eapply IH =>//.
-      by destruct Hind.
-  Qed.
-
-  Lemma upto_stutter_after_None {btr str} n:
-    upto_stutter btr str ->
-    after n str = None ->
-    ∃ n', after n' btr = None.
-  Proof.
-    have Hw: ∀ (P: nat -> Prop), (∃ n, P (S n)) -> (∃ n, P n).
-    { intros P [x ?]. by exists (S x). }
-    revert btr str. induction n as [|n IH]; intros btr str Hupto Hafter.
-    { exists 0. done. }
-    revert Hafter. punfold Hupto. induction Hupto as
-        [s|btr str s ℓ HUl HUs1 HUs2 Hind IHH|btr str s ℓ s' ℓ' ?? Hind].
-    - intros Hafter. by exists 1.
-    - intros Hafter.
-      apply Hw. simpl. by apply IHH.
-    - intros Hafter. simpl in Hafter.
-      apply Hw. simpl. eapply IH =>//.
-      by destruct Hind.
-  Qed.
-
-  Program Fixpoint destutter_once_step N Ψ (btr: trace St L) :
-    Ψ (trfirst btr) < N →
-    dec_unless Us Ul Ψ btr →
-    S' + (S' * L' * { btr' : trace St L | dec_unless Us Ul Ψ btr'}) :=
-    match N as n return
-          Ψ (trfirst btr) < n →
-          dec_unless Us Ul Ψ btr →
-          S' + (S' * L' * { btr' : trace St L | dec_unless Us Ul Ψ btr'})
-    with
-    | O => λ Hlt _, False_rect _ (Nat.nlt_0_r _ Hlt)
-    | S N' =>
-      λ Hlt Hdec,
-      match btr as z return btr = z → S' + (S' * L' * { btr' : trace St L | dec_unless Us Ul Ψ btr'}) with
-      | tr_singl s => λ _, inl (Us s)
-      | tr_cons s l btr' =>
-        λ Hbtreq,
-        match Ul l as z return Ul l = z → S' + (S' * L' * { btr' : trace St L | dec_unless Us Ul Ψ btr'}) with
-        | Some l' => λ _, inr (Us s, l', exist _ btr' _)
-        | None => λ HUll, destutter_once_step N' Ψ btr' _ _
-        end eq_refl
-      end eq_refl
-    end.
-  Next Obligation.
-  Proof.
-    intros _ Ψ btr N' Hlt Hdec s l btr' -> l' HUll; simpl.
-    eapply dec_unless_next; done.
-  Qed.
-  Next Obligation.
-  Proof.
-    intros _ Ψ btr N' Hlt Hdec s l btr' -> HUll; simpl in *.
-    pose proof (Hdec 0) as [[? ?]|[? ?]]; [congruence|lia].
-  Qed.
-  Next Obligation.
-  Proof.
-    intros _ Ψ btr N' Hlt Hdec s l btr' -> HUll; simpl.
-    eapply dec_unless_next; done.
-  Qed.
-
-  CoFixpoint destutter_gen Ψ N (btr: trace St L) :
-    Ψ (trfirst btr) < N ->
-    dec_unless Us Ul Ψ btr → trace S' L' :=
-    λ Hlt Hdec,
-    match destutter_once_step N Ψ btr Hlt Hdec with
-    | inl s' => tr_singl s'
-    | inr (s', l', z) => tr_cons s' l' (destutter_gen Ψ  (S (Ψ (trfirst $ proj1_sig z)))
-                                                 (proj1_sig z) (Nat.lt_succ_diag_r _) (proj2_sig z))
-    end.
-
-  Definition destutter Ψ (btr: trace St L) :
-    dec_unless Us Ul Ψ btr → trace S' L' :=
-    λ Hdec,
-    destutter_gen Ψ (S (Ψ (trfirst btr))) btr (Nat.lt_succ_diag_r _) Hdec.
-
-  Lemma destutter_same_Us N Ψ btr Hlt Hdec:
-    match destutter_once_step N Ψ btr Hlt Hdec with
-    | inl s' | inr (s', _, _) => Us (trfirst btr) = s'
-    end.
-  Proof.
-    revert btr Hlt Hdec. induction N as [|N]; first lia.
-    intros btr Hlt Hdec. simpl.
-    destruct btr as [s|s ℓ btr']; first done.
-    generalize (destutter_once_step_obligation_1 Ψ (s -[ ℓ ]-> btr') N
-                Hlt Hdec s ℓ btr' eq_refl).
-    generalize (destutter_once_step_obligation_2 Ψ (s -[ ℓ ]-> btr') N Hlt Hdec s ℓ btr' eq_refl).
-    generalize (destutter_once_step_obligation_3 Ψ (s -[ ℓ ]-> btr') N Hlt Hdec s ℓ btr' eq_refl).
-    intros HunlessNone HltNone HdecSome.
-    destruct (Ul ℓ) as [ℓ'|] eqn:Heq; cbn; first done.
-    unfold dec_unless in Hdec.
-    destruct (Hdec 0) as [[??]|[? Hsame]]; first congruence.
-    rewrite Hsame. apply IHN.
-  Qed.
-
-  Lemma destutter_spec_ind N Ψ (btr: trace St L) (Hdec: dec_unless Us Ul Ψ btr)
-    (Hlt: Ψ (trfirst btr) < N):
-    upto_stutter btr (destutter_gen Ψ N btr Hlt Hdec).
-  Proof.
-    revert N btr Hlt Hdec.
-    pcofix CH. pfold.
-    induction N.
-    { intros; lia. }
-    intros btr Hlt Hdec.
-    rewrite (trace_unfold_fold (destutter_gen _ _ _ _ _)).
-    destruct btr as [s|s ℓ btr'].
-    { simpl in *. econstructor. }
-    cbn.
-    generalize (destutter_once_step_obligation_1 Ψ (s -[ ℓ ]-> btr') N
-                Hlt Hdec s ℓ btr' eq_refl).
-    generalize (destutter_once_step_obligation_2 Ψ (s -[ ℓ ]-> btr') N Hlt Hdec s ℓ btr' eq_refl).
-    generalize (destutter_once_step_obligation_3 Ψ (s -[ ℓ ]-> btr') N Hlt Hdec s ℓ btr' eq_refl).
-    intros HunlessNone HltNone HdecSome.
-    destruct (Ul ℓ) as [ℓ'|] eqn:Heq; cbn.
-    - econstructor 3 =>//. right. apply (CH (S (Ψ $ trfirst btr'))).
-    - econstructor 2=>//.
-      + destruct (Hdec 0) as [[??]|[??]];congruence.
-      + have ?: Us s = Us (trfirst btr').
-        { destruct (Hdec 0) as [[??]|[? Hsame]]; congruence. }
-        have HH := destutter_same_Us N Ψ btr' (HltNone eq_refl) (HunlessNone eq_refl).
-        destruct (destutter_once_step N Ψ btr' (HltNone eq_refl) (HunlessNone eq_refl)) as
-            [|[[??][??]]]eqn:Heq'; simpl in *; congruence.
-      + rewrite -trace_unfold_fold.
-        specialize (IHN btr' (HltNone eq_refl) (HunlessNone eq_refl)).
-        match goal with
-          [H : context[upto_stutter_ind]  |- ?Y] => let X := type of H in
-                          suffices <-: X <-> Y; first done
-        end.
-        f_equiv.
-        rewrite {1}(trace_unfold_fold (destutter_gen _ _ _ _ _)) /= -trace_unfold_fold //.
-  Qed.
-
-  Lemma destutter_spec Ψ (btr: trace St L) (Hdec: dec_unless Us Ul Ψ btr):
-    upto_stutter btr (destutter Ψ btr Hdec).
-  Proof. eapply destutter_spec_ind. Qed.
-
-  Lemma can_destutter Ψ (btr: trace St L) (Hdec: dec_unless Us Ul Ψ btr):
-    ∃ str, upto_stutter btr str.
-  Proof. exists (destutter Ψ btr Hdec). apply destutter_spec. Qed.
-
-End destuttering.
-
 Section destuttering_auxtr.
-  Context {Mdl: FairModel}.
-  Context {Λ: language}.
-  Context {LM: LiveModel Λ Mdl}.
+  Context `{LM: LiveModel Λ M}.
 
   Context `{Countable (locale Λ)}.
 
   (* Why is [LM] needed here? *)
   Definition upto_stutter_auxtr :=
-    upto_stutter (@ls_under Λ Mdl) (Ul (LM := LM)).
+    upto_stutter (ls_under (Λ:=Λ) (M:=M)) (Ul (LM := LM)).
 
   Lemma can_destutter_auxtr extr auxtr:
     (∀ c c', locale_step (Λ := Λ) c None c' -> False) ->
@@ -1279,9 +715,7 @@ Section destuttering_auxtr.
 End destuttering_auxtr.
 
 Section model_traces.
-  Context {M: FairModel}.
-  Context {Λ: language}.
-  Context {LM: LiveModel Λ M}.
+  Context `{LM: LiveModel Λ M}.
   Context `{Countable (locale Λ)}.
 
   Definition mtrace := trace M (option M.(fmrole)).
@@ -1330,7 +764,7 @@ Section model_traces.
   Hint Resolve mtrace_valid_mono : paco.
 
   Lemma upto_stutter_mono' :
-    monotone2 (upto_stutter_ind (@ls_under Λ M) (@Ul M Λ LM)).
+    monotone2 (upto_stutter_ind (ls_under (Λ:=Λ) (M:=M)) (Ul (LM:=LM))).
   Proof.
     unfold monotone2. intros x0 x1 r r' IN LE.
     induction IN; try (econstructor; eauto; done).
@@ -1365,16 +799,14 @@ Global Hint Resolve fair_model_trace_cons: core.
 
 Arguments mtrace : clear implicits.
 
-Section upto_stutter_preserves_fairness_and_terminaison.
-  Context {M: FairModel}.
-  Context {Λ: language}.
-  Context {LM: LiveModel Λ M}.
+Section upto_stutter_preserves_fairness_and_termination.
+  Context `{LM: LiveModel Λ M}.
   Context `{Countable (locale Λ)}.
 
   Notation upto_stutter_aux := (upto_stutter (ls_under (Λ := Λ)) (Ul (Λ := Λ) (LM := LM))).
 
   Lemma upto_stutter_mono'' : (* TODO fix this proliferation *)
-    monotone2 (upto_stutter_ind (@ls_under Λ M) (@Ul M Λ LM)).
+    monotone2 (upto_stutter_ind (ls_under (Λ:=Λ) (M:=M)) (Ul (LM:=LM))).
   Proof.
     unfold monotone2. intros x0 x1 r r' IN LE.
     induction IN; try (econstructor; eauto; done).
@@ -1453,23 +885,6 @@ Section upto_stutter_preserves_fairness_and_terminaison.
     eexists; done.
   Qed.
 
-End upto_stutter_preserves_fairness_and_terminaison.
-
-(* Classical *)
-
-Require Import Coq.Logic.Classical.
-Section infinite_or_finite.
-  Context {St L: Type}.
-
-  Lemma infinite_or_finite (tr: trace St L):
-    infinite_trace tr ∨ terminating_trace tr.
-  Proof.
-    destruct (classic (infinite_trace tr)) as [|Hni]; first by eauto.
-    rewrite /infinite_trace in Hni.
-    apply not_all_ex_not in Hni. destruct Hni as [n Hni%eq_None_not_Some].
-    by right; exists n.
-  Qed.
-
-End infinite_or_finite.
+End upto_stutter_preserves_fairness_and_termination.
 
 Global Hint Resolve mtrace_valid_mono : paco.
